theories/zoo/language/prophecy_erasure.v
@@ -1,10 +1,12 @@
+From stdpp Require Import
+  gmap.
+
 From zoo Require Import
   prelude.
-From zoo.iris.program_logic Require Export
-  adequacy.
+From zoo.common Require Import
+  list.
 From zoo.language Require Export
-  tactics
-  notations.
+  tactics.
 From zoo Require Import
   options.
 
@@ -15,11 +17,129 @@ Implicit Types lit : literal.
 Implicit Types e : expr.
 Implicit Types es : list expr.
 Implicit Types v w : val.
+Implicit Types rec : recursive.
 Implicit Types k : ectxi.
 Implicit Types K : ectx.
 Implicit Types h : gmap location val.
 Implicit Types σ : state.
 Implicit Types ρ : config zoo.
+
+Definition literal_wf lit :=
+  match lit with
+  | LitPoison =>
+      False
+  | _ =>
+      True
+  end.
+
+Fixpoint expr_wf e :=
+  match e with
+  | Val v =>
+      val_wf v
+  | Var _ =>
+      True
+  | Rec _ _ e =>
+      expr_wf e
+  | App e1 e2 =>
+      expr_wf e1 ∧
+      expr_wf e2
+  | Let _ e1 e2 =>
+      expr_wf e1 ∧
+      expr_wf e2
+  | Unop _ e =>
+      expr_wf e
+  | Binop _ e1 e2 =>
+      expr_wf e1 ∧
+      expr_wf e2
+  | Equal e1 e2 =>
+      expr_wf e1 ∧
+      expr_wf e2
+  | If e0 e1 e2 =>
+      expr_wf e0 ∧
+      expr_wf e1 ∧
+      expr_wf e2
+  | For e1 e2 e3 =>
+      expr_wf e1 ∧
+      expr_wf e2 ∧
+      expr_wf e3
+  | Alloc e1 e2 =>
+      expr_wf e1 ∧
+      expr_wf e2
+  | Block _ _ es =>
+      Forall' expr_wf es
+  | Reveal e =>
+      expr_wf e
+  | Match e0 _ e1 brs =>
+      expr_wf e0 ∧
+      expr_wf e1 ∧
+      Forall' (λ br, expr_wf br.2) brs
+  | GetTag e =>
+      expr_wf e
+  | GetSize e =>
+      expr_wf e
+  | Load e1 e2 =>
+      expr_wf e1 ∧
+      expr_wf e2
+  | Store e1 e2 e3 =>
+      expr_wf e1 ∧
+      expr_wf e2 ∧
+      expr_wf e3
+  | Xchg e1 e2 =>
+      expr_wf e1 ∧
+      expr_wf e2
+  | CAS e0 e1 e2 =>
+      expr_wf e0 ∧
+      expr_wf e1 ∧
+      expr_wf e2
+  | FAA e1 e2 =>
+      expr_wf e1 ∧
+      expr_wf e2
+  | Fork e =>
+      expr_wf e
+  | Proph =>
+      True
+  | Resolve e0 e1 e2 =>
+      expr_wf e0 ∧
+      expr_wf e1 ∧
+      expr_wf e2
+  end
+with val_wf v :=
+  match v with
+  | ValLit lit =>
+      literal_wf lit
+  | ValRecs _ recs =>
+      Forall' (λ rec, expr_wf rec.2) recs
+  | ValBlock _ _ vs =>
+      Forall' val_wf vs
+  end.
+
+Definition exprs_wf :=
+  Forall expr_wf.
+
+Definition state_wf σ :=
+  map_Forall (λ _, val_wf) σ.(state_heap).
+
+Definition config_wf ρ :=
+  exprs_wf ρ.1 ∧
+  state_wf ρ.2.
+
+Lemma fill_item_wf_inv k e :
+  expr_wf (fill_item k e) →
+  expr_wf e.
+Proof.
+  intros H.
+  induction k; try naive_solver.
+  rewrite /= Forall'_Forall in H.
+  list_simplifier. done.
+Qed.
+Lemma fill_wf_inv K e :
+  expr_wf (fill K e) →
+  expr_wf e.
+Proof.
+  induction K as [| k K IH] using rev_ind; first done.
+  rewrite fill_app /=.
+  intros ?%fill_item_wf_inv%IH. done.
+Qed.
 
 Definition erase_literal lit :=
   match lit with
@@ -30,7 +150,7 @@ Definition erase_literal lit :=
   end.
 
 Definition erase_resolve e0 e1 e2 : expr :=
-  (e2, e1, e0).<2>.
+  Load (Block Immutable 0 [e0; e1; e2]) (Val $ ValInt 0).
 Fixpoint erase_expr e :=
   match e with
   | Val v =>
@@ -126,7 +246,7 @@ Fixpoint erase_expr e :=
       Fork
         (erase_expr e)
   | Proph =>
-      (fun: <> => #LitPoison)%V ()%V
+      App (Val $ ValFun BAnon (Val ValPoison)) (Val ValUnit)
   | Resolve e0 e1 e2 =>
       erase_resolve
         (erase_expr e0)
@@ -151,48 +271,11 @@ with erase_val v :=
 #[global] Arguments erase_expr !_ / : assert.
 #[global] Arguments erase_val !_ / : assert.
 
+Definition erase_recursive rec :=
+  (rec.1, erase_expr rec.2).
+
 Definition erase_exprs es :=
   erase_expr <$> es.
-
-Lemma erase_val_subst x v w :
-  erase_expr (subst x v w) = subst x (erase_val v) (erase_val w).
-Proof.
-  done.
-Qed.
-Lemma erase_expr_subst x v e :
-  erase_expr (subst x v e) = subst x (erase_val v) (erase_expr e).
-Proof.
-  move: e. fix IH 1. destruct e.
-  all: simpl.
-  all: try repeat destruct (_ =? _)%string.
-  all: try repeat destruct (binder_eqb _ _).
-  all: rewrite ?IH; auto.
-  all:
-    try select (list expr) ltac:(fun es =>
-      induction es; first done;
-      naive_solver congruence
-    ).
-  all:
-    try select (list branch) ltac:(fun brs =>
-      f_equal;
-      induction brs; first done;
-      simpl;
-      try repeat destruct (existsb _ _);
-      try repeat destruct (binder_eqb _ _);
-      rewrite ?IH; f_equal; done
-    ).
-Qed.
-
-Lemma erase_expr_subst' x v e :
-  erase_expr (subst' x v e) = subst' x (erase_val v) (erase_expr e).
-Proof.
-  destruct x; eauto using erase_expr_subst.
-Qed.
-Lemma erase_val_subst' x v w :
-  erase_expr (subst x v w) = subst x (erase_val v) (erase_val w).
-Proof.
-  destruct x; eauto using erase_val_subst.
-Qed.
 
 Fixpoint erase_ectxi k : ectx :=
   match k with
@@ -200,6 +283,8 @@ Fixpoint erase_ectxi k : ectx :=
       [CtxApp1 (erase_val v2)]
   | CtxApp2 e1 =>
       [CtxApp2 (erase_expr e1)]
+  | CtxLet x e2 =>
+      [CtxLet x (erase_expr e2)]
   | CtxUnop op =>
       [CtxUnop op]
   | CtxBinop1 op v2 =>
@@ -212,30 +297,34 @@ Fixpoint erase_ectxi k : ectx :=
       [CtxEqual2 (erase_expr e1)]
   | CtxIf e1 e2 =>
       [CtxIf (erase_expr e1) (erase_expr e2)]
-  | CtxConstr tag vs es =>
-      [CtxConstr tag (erase_val <$> vs) (erase_expr <$> es)]
-  | CtxProj proj =>
-      [CtxProj proj]
-  | CtxMatch x e1 brs =>
-      [CtxMatch x (erase_expr e1) ((λ br, (br.1, erase_expr br.2)) <$> brs)]
-  | CtxReveal =>
-      [CtxReveal]
   | CtxFor1 e2 e3 =>
       [CtxFor1 (erase_expr e2) (erase_expr e3)]
   | CtxFor2 v1 e3 =>
       [CtxFor2 (erase_val v1) (erase_expr e3)]
-  | CtxRecord vs es =>
-      [CtxRecord (erase_val <$> vs) (erase_expr <$> es)]
   | CtxAlloc1 v2 =>
       [CtxAlloc1 (erase_val v2)]
   | CtxAlloc2 e1 =>
       [CtxAlloc2 (erase_expr e1)]
-  | CtxLoad =>
-      [CtxLoad]
-  | CtxStore1 v2 =>
-      [CtxStore1 (erase_val v2)]
-  | CtxStore2 e1 =>
-      [CtxStore2 (erase_expr e1)]
+  | CtxBlock mut tag es vs =>
+      [CtxBlock mut tag (erase_expr <$> es) (erase_val <$> vs)]
+  | CtxReveal =>
+      [CtxReveal]
+  | CtxMatch x e1 brs =>
+      [CtxMatch x (erase_expr e1) ((λ br, (br.1, erase_expr br.2)) <$> brs)]
+  | CtxGetTag =>
+      [CtxGetTag]
+  | CtxGetSize =>
+      [CtxGetSize]
+  | CtxLoad1 v2 =>
+      [CtxLoad1 (erase_val v2)]
+  | CtxLoad2 e1 =>
+      [CtxLoad2 (erase_expr e1)]
+  | CtxStore1 v2 v3 =>
+      [CtxStore1 (erase_val v2) (erase_val v3)]
+  | CtxStore2 e1 v3 =>
+      [CtxStore2 (erase_expr e1) (erase_val v3)]
+  | CtxStore3 e1 e2 =>
+      [CtxStore3 (erase_expr e1) (erase_expr e2)]
   | CtxXchg1 v2 =>
       [CtxXchg1 (erase_val v2)]
   | CtxXchg2 e1 =>
@@ -252,11 +341,11 @@ Fixpoint erase_ectxi k : ectx :=
       [CtxFAA2 (erase_expr e1)]
   | CtxResolve0 k v1 v2 =>
       erase_ectxi k ++
-      [CtxConstr 0 [erase_val v2; erase_val v1] []; CtxProj 2]
+      [CtxBlock Immutable 0 [] [erase_val v1; erase_val v2]; CtxLoad1 (ValInt (Z.of_nat 0))]
   | CtxResolve1 e0 v2 =>
-      [CtxConstr 0 [erase_val v2] [erase_expr e0]; CtxProj 2]
+      [CtxBlock Immutable 0 [erase_expr e0] [erase_val v2]; CtxLoad1 (ValInt (Z.of_nat 0))]
   | CtxResolve2 e0 e1 =>
-      [CtxConstr 0 [] [erase_expr e1; erase_expr e0]; CtxProj 2]
+      [CtxBlock Immutable 0 [erase_expr e0; erase_expr e1] []; CtxLoad1 (ValInt (Z.of_nat 0))]
   end.
 
 Definition erase_ectx K : ectx :=
@@ -266,27 +355,44 @@ Definition erase_heap h :=
   erase_val <$> h.
 
 Definition erase_state σ :=
-  {|state_heap := erase_heap (state_heap σ) ;
+  {|state_headers := σ.(state_headers) ;
+    state_heap := erase_heap σ.(state_heap) ;
     state_prophets := ∅ ;
   |}.
 
-Definition erase_cfg ρ : config zoo :=
-  (erase_exprs ρ.1, erase_state ρ.2).
-
-Lemma erase_to_val e v :
-  to_val (erase_expr e) = Some v →
-    ∃ v',
-    to_val e = Some v' ∧
-    erase_val v' = v.
+Lemma erase_to_val e 𝑣 :
+  to_val (erase_expr e) = Some 𝑣 →
+    ∃ v,
+    to_val e = Some v ∧
+    erase_val v = 𝑣.
 Proof.
   destruct e; naive_solver.
 Qed.
-
+Lemma erase_expr_val_inv e 𝑣 :
+  erase_expr e = Val 𝑣 →
+    ∃ v,
+    e = Val v ∧
+    𝑣 = erase_val v.
+Proof.
+  destruct e; naive_solver.
+Qed.
 Lemma erase_not_val e :
   to_val e = None →
   to_val (erase_expr e) = None.
 Proof.
   destruct e; done.
+Qed.
+Lemma erase_exprs_vals es 𝑣s :
+  erase_exprs es = of_vals 𝑣s →
+    ∃ vs,
+    es = of_vals vs ∧
+    𝑣s = erase_val <$> vs.
+Proof.
+  move: 𝑣s. induction es as [| e es IH] => 𝑣s H.
+  all: destruct 𝑣s as [| 𝑣 𝑣s]; try done.
+  - eauto.
+  - injection H as [= (v & -> & ->)%erase_expr_val_inv (vs & -> & ->)%IH].
+    exists (v :: vs). done.
 Qed.
 
 Lemma erase_ectx_app K1 K2 :
@@ -295,771 +401,222 @@ Proof.
   rewrite /erase_ectx bind_app //.
 Qed.
 
-Lemma erase_expr_fill K e :
+Lemma erase_fill_item k e :
+  erase_expr (fill_item k e) = fill (erase_ectxi k) (erase_expr e).
+Proof.
+  induction k.
+  all: rewrite //=.
+  - rewrite fmap_app fmap_cons /of_vals -!list_fmap_compose //.
+  - rewrite fill_app IHk //.
+Qed.
+Lemma erase_fill K e :
   erase_expr (fill K e) = fill (erase_ectx K) (erase_expr e).
 Proof.
-  move: e. induction K as [| k K IH] using rev_ind => e //.
-  rewrite !erase_ectx_app !fill_app /= -{}IH.
-  induction k.
-  all: rewrite ?fill_app /= /erase_resolve.
-  all: auto 10 with f_equal.
-  all: rewrite fmap_app /of_vals -!list_fmap_compose //.
+  move: e. induction K as [| k K IH] using rev_ind => e; first done.
+  rewrite erase_ectx_app !fill_app /= erase_fill_item IH //.
 Qed.
 
-(* Lemma val_unboxed_erased v : *)
-(*   val_unboxed (erase_val v) ↔ val_unboxed v. *)
-(* Proof. *)
-(*   destruct v; rewrite /= /literal_unboxed; repeat (done || simpl; case_match). *)
-(* Qed. *)
-(* Lemma val_comparable_erase v1 v2 : *)
-(*   val_comparable (erase_val v1) (erase_val v2) ↔ *)
-(*   val_comparable v1 v2. *)
-(* Proof. *)
-(*   rewrite /val_comparable !val_unboxed_erased. done. *)
-(* Qed. *)
-(* Lemma erase_val_inj_iff v1 v2 : *)
-(*   val_comparable v1 v2 → *)
-(*   erase_val v1 = erase_val v2 ↔ v1 = v2. *)
-(* Proof. *)
-(*   destruct v1, v2; rewrite /= /literal_unboxed; *)
-(*     repeat (done || (by intros [[] | []]) || simpl; case_match). *)
-(* Qed. *)
-
-Lemma eval_unop_erase op v v' :
-  eval_unop op (erase_val v) = Some v' ↔
-    ∃ w,
-    eval_unop op v = Some w ∧
-    erase_val w = v'.
+Lemma erase_fill_inv e 𝐾 𝑒 𝜎 :
+  (* not_stuck e σ → *)
+  base_reducible 𝑒 𝜎 →
+  erase_expr e = fill 𝐾 𝑒 →
+    ∃ K e',
+    𝐾 = erase_ectx K ∧
+    𝑒 = erase_expr e' ∧
+    e = fill K e'.
 Proof.
-  destruct op, v as [[] | |]; naive_solver.
+  intros H𝑒.
+  move: e. induction 𝐾 as [| 𝑘 𝐾 IH] using rev_ind => e Heq.
+  { eexists [], _. done. }
+  rewrite fill_app /= in Heq.
+  destruct 𝑘, e.
+  all: try done.
+  all: simplify.
+  all:
+    repeat
+      match goal with
+      | H: erase_expr _ = Val _ |- _ =>
+          apply erase_expr_val_inv in H as (? & -> & ->)
+      | H: erase_expr _ = fill _ _ |- _ =>
+          apply IH in H as (? & ? & -> & -> & ->)
+      end.
+  all:
+    try solve [
+      match goal with
+      | |- context [_ ++ [?k _ _]] =>
+          eexists (_ ++ [k _ _])
+      | |- context [_ ++ [?k _]] =>
+          eexists (_ ++ [k _])
+      | |- context [_ ++ [?k]] =>
+          eexists (_ ++ [k])
+      end;
+      eexists;
+      rewrite erase_ectx_app fill_app //
+    ].
+  - destruct (rev_elim 𝐾) as [-> | (𝐾' & 𝑘 & ->)].
+    + apply base_reducible_not_val in H𝑒. naive_solver.
+    + rewrite fill_app /= in Heq. destruct 𝑘; done.
+  - destruct (rev_elim 𝐾) as [-> | (𝐾' & 𝑘 & ->)].
+    + apply base_reducible_not_val in H𝑒. naive_solver.
+    + rewrite fill_app /= in H. destruct 𝑘; done.
+  - select (erase_expr <$> _ = _) (fun Heq =>
+      apply fmap_app_cons_inv in Heq as (es1 & e & es2 & -> & -> & (K & e' & -> & -> & ->)%symmetry%IH & (? & -> & ->)%symmetry%erase_exprs_vals)
+    ).
+    eexists (_ ++ [CtxBlock _ _ _ _]), _.
+    rewrite erase_ectx_app fill_app //.
+  - rewrite /erase_resolve /= in Heq.
+    simplify.
+    destruct (rev_elim 𝐾) as [-> | (𝐾' & 𝑘 & ->)].
+    + assert (∃ σ, reducible (Resolve e1 e2 e3) σ) as (σ & He) by admit.
+      simplify.
+      destruct H𝑒 as (𝜅 & 𝑒' & 𝜎' & 𝑒s & H𝑠𝑡𝑒𝑝).
+      invert H𝑠𝑡𝑒𝑝.
+      apply (erase_exprs_vals [e1; e2; e3]) in H as (? & ? & ->).
+      do 3 (destruct x as [| ? x]; first done).
+      simplify.
+      destruct He as (κ & e' & σ' & es & [? ? ? ? ? Hstep]).
+      simplify.
+      admit.
+    + rewrite fill_app /= in Heq.
+      destruct 𝑘; try done.
+      simplify.
+      (* destruct es. *)
+      admit.
+  - injection Heq as [= _ Heq].
+    edestruct (fill_val 𝐾 𝑒). { rewrite /= -Heq //. }
+    apply base_reducible_not_val in H𝑒. naive_solver.
+Admitted.
+Lemma erase_base_step_inv e1 σ1 𝜅 𝑒2 𝜎2 𝑒s :
+  expr_wf e1 →
+  state_wf σ1 →
+  base_step (erase_expr e1) (erase_state σ1) 𝜅 𝑒2 𝜎2 𝑒s →
+    ∃ κ e2 σ2 es,
+    expr_wf e2 ∧
+    state_wf σ2 ∧
+    exprs_wf es ∧
+    base_step e1 σ1 κ e2 σ2 es ∧
+    rtc pure_step 𝑒2 (erase_expr e2) ∧
+    𝜎2 = erase_state σ2 ∧
+    𝑒s = erase_exprs es.
+Proof.
+Admitted.
+Lemma erase_prim_step_inv e1 σ1 𝜅 𝑒2 𝜎2 𝑒s :
+  expr_wf e1 →
+  state_wf σ1 →
+  prim_step (erase_expr e1) (erase_state σ1) 𝜅 𝑒2 𝜎2 𝑒s →
+    ∃ κ e2 σ2 es,
+    expr_wf e2 ∧
+    state_wf σ2 ∧
+    exprs_wf es ∧
+    prim_step e1 σ1 κ e2 σ2 es ∧
+    rtc pure_step 𝑒2 (erase_expr e2) ∧
+    𝜎2 = erase_state σ2 ∧
+    𝑒s = erase_exprs es.
+Proof.
+  intros He1 Hσ1 [𝐾 𝑒1' 𝑒2' Heq -> H𝑠𝑡𝑒𝑝].
+  eapply erase_fill_inv in Heq as (K & e1' & -> & -> & ->).
+  2: eauto with zoo.
+  apply erase_base_step_inv in H𝑠𝑡𝑒𝑝 as (κ & e2' & σ2 & es & He2' & Hσ2 & Hes & Hstep & Hrel & -> & ->); first last.
+  { done. }
+  { eapply fill_wf_inv. done. }
+  exists κ, (fill K e2'), σ2, es. split_and!; try done.
+  - admit.
+  - apply base_step_fill_prim_step. done.
+  - admit.
+Admitted.
+
+Definition erase_relation ρ 𝜌 :=
+  config_wf ρ ∧
+  Forall2 (λ e 𝑒, rtc pure_step 𝑒 (erase_expr e)) ρ.1 𝜌.1 ∧
+  𝜌.2 = erase_state ρ.2.
+Lemma erase_relation_step ρ1 𝜌1 𝜌2 :
+  erase_relation ρ1 𝜌1 →
+  silent_step 𝜌1 𝜌2 →
+    ∃ ρ2,
+    erase_relation ρ2 𝜌2 ∧
+    rtc silent_step ρ1 ρ2.
+Proof.
+  destruct ρ1 as (es1, σ1), 𝜌1 as (𝑒s1, 𝜎1).
+  intros ((Hes1 & Hσ1) & Hrel & ?) (𝜅 & (i & 𝑒1 & 𝑒2 & 𝜎2 & 𝑒s & H𝑠𝑡𝑒𝑝 & H𝑒s1_lookup & ->)).
+  simplify.
+  opose proof* Forall2_lookup_r as (e1 & Hes1_lookup & H𝑠𝑡𝑒𝑝s); [done.. |].
+  apply rtc_inv in H𝑠𝑡𝑒𝑝s as [-> | (𝑒1' & H𝑠𝑡𝑒𝑝_ & H𝑠𝑡𝑒𝑝s)].
+  - opose proof* Forall_lookup_1 as He1; [done.. |].
+    opose proof* erase_prim_step_inv as (κ & e2 & σ2 & es & He2 & Hσ2 & Hes & Hstep & H𝑠𝑡𝑒𝑝s & -> & Heq); [done.. |]. subst 𝑒s.
+    exists (<[i := e2]> es1 ++ es, σ2). split.
+    + split_and!; first split; try done.
+      * apply Forall_app_2; last done. apply Forall_insert; done.
+      * apply Forall2_app.
+        -- apply Forall2_insert; done.
+        -- apply Forall2_fmap_r, Forall_Forall2_diag, Forall_true.
+           eauto using rtc.
+    + apply rtc_once. exists κ, i, e1, e2, σ2, es. done.
+  - eapply pure_step_det in H𝑠𝑡𝑒𝑝 as (-> & -> & -> & ->); last done.
+    rewrite right_id.
+    exists (es1, σ1). split; last done. split_and!; try done.
+    eapply Forall2_insert_r; done.
+Qed.
+Lemma erase_relation_steps ρ1 𝜌1 𝜌2 :
+  erase_relation ρ1 𝜌1 →
+  rtc silent_step 𝜌1 𝜌2 →
+    ∃ ρ2,
+    erase_relation ρ2 𝜌2 ∧
+    rtc silent_step ρ1 ρ2.
+Proof.
+  intros Hrel1 H𝑠𝑡𝑒𝑝s.
+  move: ρ1 Hrel1. induction H𝑠𝑡𝑒𝑝s as [| 𝜌1 𝜌2 𝜌3 H𝑠𝑡𝑒𝑝 H𝑠𝑡𝑒𝑝s IH] => ρ1 Hrel1.
+  - naive_solver.
+  - eapply erase_relation_step in H𝑠𝑡𝑒𝑝 as (ρ2 & (ρ3 & Hrel3 & Hsteps2)%IH & Hsteps1); last done.
+    eexists. split; first done. etrans; done.
 Qed.
 
-Lemma eval_binop_erase op v1 v2 v' :
-  eval_binop op (erase_val v1) (erase_val v2) = Some v' ↔
-    ∃ w,
-    eval_binop op v1 v2 = Some w ∧
-    erase_val w = v'.
+Lemma erase_base_reducible e σ :
+  base_reducible e σ →
+  reducible (erase_expr e) (erase_state σ).
 Proof.
-  destruct v1 as [[] | |]; try naive_solver;
-  destruct v2 as [[] | |]; try naive_solver;
-  destruct op; naive_solver.
-
-  (* rewrite /bin_op_eval /bin_op_eval_int /bin_op_eval_bool /bin_op_eval_loc; *)
-  (*   split; [intros ?|intros (?&?&?)]; *)
-  (*     repeat (case_match; simplify_eq/=); eauto. *)
-  (* - eexists _; split; eauto; simpl. *)
-  (*   erewrite bool_decide_ext; first by eauto. *)
-  (*   rewrite erase_val_inj_iff; done. *)
-  (* - by assert (val_comparable v1 v2) by by apply val_comparable_erase. *)
-  (* - by erewrite bool_decide_ext; last apply erase_val_inj_iff. *)
-  (* - by assert (val_comparable (erase_val v1) (erase_val v2)) *)
-  (*     by by apply val_comparable_erase. *)
+  intros (κ & e2 & σ2 & es & Hstep).
+  invert Hstep.
+  all:
+    try solve [
+      eexists _, _, _, _, [] _ _;
+      constructor
+    ].
+Admitted.
+Lemma erase_reducible e σ :
+  reducible e σ →
+  reducible (erase_expr e) (erase_state σ).
+Proof.
+  intros (κ & e2 & σ2 & es & [K e1' e2' -> -> Hstep]).
+  rewrite erase_fill.
+  apply reducible_fill, erase_base_reducible.
+  eauto with zoo.
+Qed.
+Lemma erase_not_stuck e σ :
+  not_stuck e σ →
+  not_stuck (erase_expr e) (erase_state σ).
+Proof.
+  intros [(v & <-%of_to_val) | Hstep].
+  - apply val_not_stuck. done.
+  - apply reducible_not_stuck, erase_reducible. done.
 Qed.
 
-Lemma lookup_erase_heap_None h l :
-  erase_heap h !! l = None ↔ h !! l = None.
+Lemma erase_safe e σ :
+  expr_wf e →
+  state_wf σ →
+  safe ([e], σ) →
+  safe ([erase_expr e], erase_state σ).
 Proof.
-  rewrite lookup_fmap; destruct (h !! l); done.
-Qed.
-
-Lemma lookup_erase_heap h l :
-  erase_heap h !! l = erase_val <$> h !! l.
-Proof.
-  apply lookup_fmap.
-Qed.
-
-Lemma erase_heap_insert h l v :
-  erase_heap (<[l := v]> h) = <[l := erase_val v]> (erase_heap h).
-Proof.
-  apply fmap_insert.
-Qed.
-
-Lemma fmap_heap_array (f : val → val) l vs :
-  f <$> heap_array l vs = heap_array l (f <$> vs).
-Proof.
-  move: l. induction vs as [| v vs IH] => l.
-  - apply fmap_empty.
-  - rewrite fmap_insert IH //.
-Qed.
-
-Lemma erase_heap_array l vs h :
-  erase_heap (heap_array l vs ∪ h) =
-  heap_array l (erase_val <$> vs) ∪ erase_heap h.
-Proof.
-  apply map_eq => l'.
-  rewrite lookup_fmap !lookup_union -fmap_heap_array !lookup_fmap.
-  destruct (heap_array l vs !! l'), (h !! l'); done.
-Qed.
-
-Lemma erase_state_init l vs σ :
-  erase_state (state_init_heap l vs σ) =
-  state_init_heap l (erase_val <$> vs) (erase_state σ).
-Proof.
-  rewrite /erase_state erase_heap_array //.
-Qed.
-
-Definition base_steps_to_erasure_of e1 σ1 e2 σ2 es :=
-  ∃ κ' e2' σ2' es' ϕ,
-  base_step e1 σ1 κ' e2' σ2' es' ϕ ∧
-  erase_expr e2' = e2 ∧
-  erase_state σ2' = σ2 ∧
-  erase_exprs es' = es.
-
-Lemma erased_base_step_base_step_rec f x e v σ :
-  base_steps_to_erasure_of
-    ((rec: f x => e)%V v)
-    σ
-    (subst' f (rec: f x => erase_expr e) $ subst' x (erase_val v) $ erase_expr e)
-    (erase_state σ)
-    [].
-Proof.
-  repeat econstructor. rewrite !erase_expr_subst' //.
-Qed.
-Lemma erased_base_step_base_step_Proph σ :
-  base_steps_to_erasure_of
-    Proph
-    σ
-    #LitPoison
-    (erase_state σ)
-    [].
-Proof.
-  repeat eexists _. split; [apply base_step_proph' | done].
-Qed.
-Lemma erased_base_step_base_step_Alloc n v σ l :
-  (0 < n)%Z →
-  ( ∀ i : Z,
-    (0 ≤ i < n)%Z →
-    erase_heap (state_heap σ) !! (l +ₗ i) = None
-  ) →
-  base_steps_to_erasure_of
-    (Alloc #n v)
-    σ
-    #l
-    (state_init_heap l (replicate (Z.to_nat n) (erase_val v)) (erase_state σ))
-    [].
-Proof.
-  repeat eexists _. split_and!.
-  - econstructor; first done.
-    setoid_rewrite <- lookup_erase_heap_None. done.
-  - done.
-  - rewrite erase_state_init fmap_replicate //.
-  - done.
-Qed.
-Lemma erased_base_step_base_step_Load l σ v :
-  erase_heap (state_heap σ) !! l = Some v →
-  base_steps_to_erasure_of
-    (!#l)
-    σ
-    v
-    (erase_state σ)
-    [].
-Proof.
-  intros Hl.
-  rewrite lookup_erase_heap in Hl.
-  destruct (state_heap σ !! l) eqn:?; simplify.
-  repeat eexists _; split; first econstructor; done.
-Qed.
-Lemma erased_base_step_base_step_Xchg l v w σ :
-  erase_heap (state_heap σ) !! l = Some v →
-  base_steps_to_erasure_of
-    (Xchg #l w)
-    σ
-    v
-    {|state_heap := <[l := erase_val w]> (erase_heap (state_heap σ)) ;
-      state_prophets := ∅ ;
-    |}
-    [].
-Proof.
-  intros Hl.
-  rewrite lookup_erase_heap in Hl.
-  destruct (state_heap σ !! l) eqn:?; simplify.
-  repeat eexists _; split_and!; first econstructor; try done.
-  rewrite /erase_state erase_heap_insert //.
-Qed.
-Lemma erased_base_step_base_step_Store l v w σ :
-  erase_heap (state_heap σ) !! l = Some v →
-  base_steps_to_erasure_of
-    (#l <- w)
-    σ
-    ()
-    {|state_heap := <[l := erase_val w]> (erase_heap (state_heap σ)) ;
-      state_prophets := ∅ ;
-    |}
-    [].
-Proof.
-  intros Hl.
-  rewrite lookup_erase_heap in Hl.
-  destruct (state_heap σ !! l) eqn:?; simplify.
-  repeat eexists _; split_and!; first econstructor; try done.
-  rewrite /erase_state erase_heap_insert //.
-Qed.
-(* Lemma erased_base_step_base_step_CAS l v w σ vl : *)
-(*   erase_heap (heap σ) !! l = Some (Some vl) → *)
-(*   val_comparable vl (erase_val v) → *)
-(*   base_steps_to_erasure_of *)
-(*     (CAS #l v w) σ *)
-(*     (vl, #(bool_decide (vl = erase_val v)))%V *)
-(*     (if bool_decide (vl = erase_val v) *)
-(*      then {| heap := <[l:=Some $ erase_val w]> (erase_heap (heap σ)); *)
-(*              used_proph_id := ∅ |} *)
-(*      else erase_state σ) []. *)
-(* Proof. *)
-(*   intros Hl Hvl. *)
-(*   rewrite lookup_erase_heap in Hl. *)
-(*   destruct (heap σ !! l) as [[u|]|] eqn:?; simplify_eq/=. *)
-(*   rewrite -> val_comparable_erase in Hvl. *)
-(*   destruct (decide (u = v)) as [->|Hneq]. *)
-(*   - eexists _, _, _, _; simpl; split. *)
-(*     { econstructor; eauto. } *)
-(*     rewrite !bool_decide_eq_true_2; eauto using erase_val_inj_iff; []. *)
-(*     rewrite -?erase_heap_insert_Some. *)
-(*     split_and!; auto. *)
-(*   - eexists _, _, _, _; simpl; split. *)
-(*     { econstructor; eauto. } *)
-(*     rewrite !bool_decide_eq_false_2; eauto; []. *)
-(*     by rewrite erase_val_inj_iff. *)
-(* Qed. *)
-(*Lemma erased_base_step_base_step_FAA l n m σ :*)
-(*  erase_heap (heap σ) !! l = Some (Some #n) →*)
-(*  base_steps_to_erasure_of*)
-(*    (FAA #l #m) σ #n*)
-(*    {| heap := <[l:= Some #(n + m)]> (erase_heap (heap σ));*)
-(*       used_proph_id := ∅ |} [].*)
-(*Proof.*)
-(*  intros Hl.*)
-(*  rewrite lookup_erase_heap in Hl.*)
-(*  destruct (heap σ !! l) as [[[[]| | | |]|]|] eqn:?; simplify_eq/=.*)
-(*  repeat econstructor; first by eauto.*)
-(*  by rewrite /state_upd_heap /erase_state /= erase_heap_insert_Some.*)
-(*Qed.*)
-
-(*(** When the erased program makes a base step, so does the original program. *)*)
-(*Lemma erased_base_step_base_step e1 σ1 κ e2 σ2 efs:*)
-(*  base_step (erase_expr e1) (erase_state σ1) κ e2 σ2 efs →*)
-(*  base_steps_to_erasure_of e1 σ1 e2 σ2 efs.*)
-(*Proof.*)
-(*  intros Hhstep.*)
-(*  inversion Hhstep; simplify_eq/=;*)
-(*    repeat match goal with*)
-(*           | H : _ = erase_expr ?e |- _ => destruct e; simplify_eq/=*)
-(*           | H : _ = erase_val ?v |- _ => destruct v; simplify_eq/=*)
-(*           | H : _ = erase_base_lit ?l |- _ => destruct l; simplify_eq/=*)
-(*           | H : context [erased_new_proph] |- _ => unfold erased_new_proph in H*)
-(*           | H : un_op_eval _ (erase_val _) = Some _ |- _ =>*)
-(*             apply un_op_eval_erase in H as [? [? ?]]*)
-(*           | H : bin_op_eval _ (erase_val _) (erase_val _) = Some _ |- _ =>*)
-(*             apply bin_op_eval_erase in H as [? [? ?]]*)
-(*           | H : val_unboxed (erase_val _) |- _ =>*)
-(*             apply -> val_unboxed_erased in H*)
-(*           end; simplify_eq/=;*)
-(*    try (by repeat econstructor);*)
-(*  eauto using erased_base_step_base_step_rec,*)
-(*    erased_base_step_base_step_Proph,*)
-(*    erased_base_step_base_step_AllocN,*)
-(*    erased_base_step_base_step_Free,*)
-(*    erased_base_step_base_step_Load,*)
-(*    erased_base_step_base_step_Xchg,*)
-(*    erased_base_step_base_step_Store,*)
-(*    erased_base_step_base_step_CAS,*)
-(*    erased_base_step_base_step_FAA.*)
-(*Qed.*)
-
-(*Lemma fill_to_resolve e v1 v2 K e' :*)
-(*  to_val e' = None →*)
-(*  Resolve e v1 v2 = fill K e' →*)
-(*  K = [] ∨ ∃ K' Ki, K = K' ++ [ResolveLCtx Ki v1 v2].*)
-(*Proof.*)
-(*  intros Hnv Hrs; simpl in *.*)
-(*  assert (∀ v K, fill K e' ≠ v) as Hcontr.*)
-(*  { intros w K' Hw.*)
-(*    assert (to_val (of_val w) = to_val (fill K' e')) as He'*)
-(*        by (by rewrite Hw).*)
-(*    rewrite fill_not_val in He'; by eauto. }*)
-(*  destruct K as [|Ki K _] using rev_ind; first by left.*)
-(*  rewrite fill_app in Hrs.*)
-(*  destruct Ki; simplify_eq/=; eauto;*)
-(*    try exfalso; eapply Hcontr; eauto.*)
-(*Qed.*)
-
-(*Lemma projs_pure_steps (v0 v1 v2 : val) :*)
-(*  rtc pure_step (Fst (Fst (v0, v1, v2))) v0.*)
-(*Proof.*)
-(*  etrans; first apply (rtc_pure_step_ctx (fill [PairLCtx _; FstCtx; FstCtx])).*)
-(*  { apply rtc_once.*)
-(*    apply pure_base_step_pure_step.*)
-(*    split; first repeat econstructor.*)
-(*    intros ????? Hhstep; inversion Hhstep; simplify_eq/=; eauto. }*)
-(*  simpl.*)
-(*  etrans; first apply (rtc_pure_step_ctx (fill [FstCtx; FstCtx])).*)
-(*  { apply rtc_once.*)
-(*    apply pure_base_step_pure_step.*)
-(*    split; first repeat econstructor.*)
-(*    intros ????? Hhstep; inversion Hhstep; simplify_eq/=; eauto. }*)
-(*  simpl.*)
-(*  etrans; first apply (rtc_pure_step_ctx (fill [FstCtx])).*)
-(*  { apply rtc_once.*)
-(*    apply pure_base_step_pure_step.*)
-(*    split; first repeat econstructor.*)
-(*    intros ????? Hhstep; inversion Hhstep; simplify_eq/=; eauto. }*)
-(*  simpl.*)
-(*  apply rtc_once.*)
-(*  apply pure_base_step_pure_step.*)
-(*  split; first repeat econstructor.*)
-(*  intros ????? Hhstep; inversion Hhstep; simplify_eq/=; eauto.*)
-(*Qed.*)
-
-(*Lemma Resolve_3_vals_base_stuck v0 v1 v2 σ κ e σ' efs :*)
-(*  ¬ base_step (Resolve v0 v1 v2) σ κ e σ' efs.*)
-(*Proof.*)
-(*  intros Hhstep.*)
-(*  inversion Hhstep; simplify_eq/=.*)
-(*  apply (eq_None_not_Some (to_val (Val v0))); last eauto.*)
-(*  by eapply val_base_stuck.*)
-(*Qed.*)
-
-(*Lemma Resolve_3_vals_unsafe (v0 v1 v2 : val) σ :*)
-(*  ¬ not_stuck (Resolve v0 v1 v2) σ.*)
-(*Proof.*)
-(*  assert(∀ w K e, Val w = fill K e → is_Some (to_val e)) as Hvfill.*)
-(*  { intros ? K ? Heq; eapply (fill_val K); rewrite /= -Heq; eauto. }*)
-(*  apply not_not_stuck.*)
-(*  split; first done.*)
-(*  intros ???? [K e1' e2' Hrs Hhstep]; simplify_eq/=.*)
-(*  destruct K as [|Ki K _] using rev_ind.*)
-(*  { simplify_eq/=.*)
-(*    eapply Resolve_3_vals_base_stuck; eauto. }*)
-(*  rewrite fill_app in Hrs.*)
-(*  destruct Ki; simplify_eq/=.*)
-(*  - rename select ectx_item into Ki.*)
-(*    pose proof (fill_item_val Ki (fill K e1')) as Hnv.*)
-(*    apply fill_val in Hnv as [? Hnv]; last by rewrite -Hrs; eauto.*)
-(*    by erewrite val_base_stuck in Hnv.*)
-(*  - edestruct Hvfill as [? Heq]; eauto.*)
-(*    by erewrite val_base_stuck in Heq.*)
-(*  - edestruct Hvfill as [? Heq]; eauto.*)
-(*    by erewrite val_base_stuck in Heq.*)
-(*Qed.*)
-
-(*(** [(e1, σ1)] takes a [prim_step] to [(e2', σ2')] forking threads [efs']*)
-(* such that [σ2] is the erasure of [σ2'] and [efs] is the erasure of*)
-(* [efs']. Furthermore, [e2] takes [pure_steps] to match up with [e2].  It is*)
-(* crucial for us that [e2] takes [pure_step]s because we need to know*)
-(* that [e2] does not get stuck and that the steps are deterministic.*)
-
-(* Essentially, the main part of the erasure proof's argument is that if*)
-(* the erased program takes steps, then the original program also takes*)
-(* matching steps. This however, does not entirely hold. In cases where*)
-(* the erasure of [Resovle] takes a step, the original program*)
-(* immediately produces the value while the erased program has to still*)
-(* perform projections [Fst] to get the result (see the [Resolve] case*)
-(* of [erase_expr]). For this purpose, we prove that in those cases (and*)
-(* also in general) the erased program also takes a number of (possibly*)
-(* zero) steps so that the original and the erased programs are matched*)
-(* up again. *)*)
-(*Definition prim_step_matched_by_erased_steps e1 σ1 e2 σ2 efs :=*)
-(*  ∃ e2' σ2' κ' efs' e2'',*)
-(*    prim_step e1 σ1 κ' e2' σ2' efs' ∧ rtc pure_step e2 e2'' ∧*)
-(*    erase_expr e2' = e2'' ∧ erase_state σ2' = σ2 ∧ erase_exprs efs' = efs.*)
-
-(*Lemma prim_step_matched_by_erased_steps_ectx K e1 σ1 e2 σ2 efs :*)
-(*  prim_step_matched_by_erased_steps e1 σ1 e2 σ2 efs →*)
-(*  prim_step_matched_by_erased_steps (fill K e1) σ1 (fill (erase_ectx K) e2) σ2 efs.*)
-(*Proof.*)
-(*  intros (?&?&?&?&?&?&?&?&?&?); simplify_eq/=.*)
-(*  eexists _, _, _, _, _; repeat split.*)
-(*  - by apply fill_prim_step.*)
-(*  - rewrite erase_ectx_expr.*)
-(*    by eapply (rtc_pure_step_ctx (fill (erase_ectx K))).*)
-(*Qed.*)
-
-(*Definition is_Resolve (e : expr) :=*)
-(*  match e with Resolve _ _ _ => True | _ => False end.*)
-
-(*#[global] Instance is_Resolve_dec e : Decision (is_Resolve e).*)
-(*Proof. destruct e; solve_decision. Qed.*)
-
-(*Lemma non_resolve_prim_step_matched_by_erased_steps_ectx_item*)
-(*      Ki e1 e1' σ1 e2 σ2 efs :*)
-(*  to_val e1' = None →*)
-(*  ¬ is_Resolve e1 →*)
-(*  not_stuck e1 σ1 →*)
-(*  erase_expr e1 = fill_item Ki e1' →*)
-(*  (∀ e1, erase_expr e1 = e1' → not_stuck e1 σ1 →*)
-(*         prim_step_matched_by_erased_steps e1 σ1 e2 σ2 efs) →*)
-(*  prim_step_matched_by_erased_steps e1 σ1 (fill_item Ki e2) σ2 efs.*)
-(*Proof.*)
-(*  intros Hnv Hnr Hsf He1 IH.*)
-(*  destruct Ki; simplify_eq/=;*)
-(*    repeat*)
-(*      match goal with*)
-(*      | H : erase_expr ?e = _ |- _ => destruct e; simplify_eq/=; try done*)
-(*      | H : context [erased_new_proph] |- _ =>*)
-(*        rewrite /erased_new_proph in H; simplify_eq/=*)
-(*      | |- prim_step_matched_by_erased_steps ?e _ _ _ _ =>*)
-(*        let tac K e :=*)
-(*            lazymatch K with*)
-(*            | [] => fail*)
-(*            | _ => apply (prim_step_matched_by_erased_steps_ectx K);*)
-(*                    apply IH; [done| by eapply (not_stuck_fill_inv (fill K))]*)
-(*            end*)
-(*        in*)
-(*        reshape_expr e tac*)
-(*      end.*)
-(*Qed.*)
-
-(*Lemma prim_step_matched_by_erased_steps_ectx_item Ki K e1 e1' σ1 e2 σ2 efs κ :*)
-(*  base_step e1' (erase_state σ1) κ e2 σ2 efs →*)
-(*  not_stuck e1 σ1 →*)
-(*  erase_expr e1 = fill_item Ki (fill K e1') →*)
-(*  (∀ K' e1, length K' ≤ length K →*)
-(*     erase_expr e1 = (fill K' e1') → not_stuck e1 σ1 →*)
-(*     prim_step_matched_by_erased_steps e1 σ1 (fill K' e2) σ2 efs) →*)
-(*  prim_step_matched_by_erased_steps e1 σ1 (fill_item Ki (fill K e2)) σ2 efs.*)
-(*Proof.*)
-(*  intros Hhstp Hsf He1 IH; simpl in *.*)
-(*  (** Case split on whether e1 is a [Resolve] expression. *)*)
-(*  destruct (decide (is_Resolve e1)); last first.*)
-(*  { (** e1 is not a [Resolve] expression. *)*)
-(*    eapply non_resolve_prim_step_matched_by_erased_steps_ectx_item; [|by eauto..].*)
-(*    by eapply fill_not_val, val_base_stuck. }*)
-(*  (** e1 is a [Resolve] expression. *)*)
-(*  destruct Ki; simplify_eq/=;*)
-(*    repeat*)
-(*      match goal with*)
-(*      | H : erase_expr ?e = ?e' |- _ =>*)
-(*        progress*)
-(*          match e' with*)
-(*          | fill _ _ => idtac*)
-(*          | _ => destruct e; simplify_eq/=*)
-(*          end*)
-(*      end; try done.*)
-(*  destruct K as [|Ki K _] using rev_ind; simplify_eq/=; [|].*)
-(*  { (* case where (Fst (erase_expr e1_1, erase_expr e1_2, erase_expr e1_3)) *)*)
-(*    (*      takes a base_step; it is impossible! *)*)
-(*    by inversion Hhstp; simplify_eq. }*)
-(*  rewrite /erase_resolve fill_app /= in He1; simplify_eq/=.*)
-(*  destruct Ki; simplify_eq/=; rewrite fill_app /=.*)
-(*  destruct K as [|Ki K _] using rev_ind; simplify_eq/=; [|].*)
-(*  { (* case where (erase_expr e1_1, erase_expr e1_2, erase_expr e1_3) *)*)
-(*    (*      takes a base_step; it is impossible! *)*)
-(*    inversion Hhstp. }*)
-(*  rewrite fill_app /= in He1.*)
-(*  destruct Ki; simplify_eq/=; rewrite fill_app /=.*)
-(*  - destruct K as [|Ki K _] using rev_ind; simplify_eq/=; [|].*)
-(*    { (** [Resolve v0 v1 v2] is not safe! *)*)
-(*      inversion Hhstp; simplify_eq/=.*)
-(*      repeat*)
-(*        match goal with*)
-(*        | H : erase_expr ?e = _ |- _ => destruct e; simplify_eq/=*)
-(*        | H : _ = erase_expr ?e |- _ => destruct e; simplify_eq/=*)
-(*        end.*)
-(*      by exfalso; eapply Resolve_3_vals_unsafe. }*)
-(*    rewrite fill_app /= in He1.*)
-(*    destruct Ki; simplify_eq/=; rewrite fill_app /=.*)
-(*    + (** e1 is of the form ([Resolve] e10 e11 v0) and e11 takes a prim_step. *)*)
-(*      destruct Hsf as [[? ?]| (?&?&?&?&Hrpstp)]; first done; simpl in *.*)
-(*      inversion Hrpstp as [??? Hrs ? Hhstp']; simplify_eq/=.*)
-(*      repeat*)
-(*        match goal with*)
-(*        | H : erase_expr ?e = ?e' |- _ =>*)
-(*          progress*)
-(*            match e' with*)
-(*            | fill _ _ => idtac*)
-(*            | _ => destruct e; simplify_eq/=*)
-(*            end*)
-(*        end.*)
-(*      edestruct fill_to_resolve as [?|[K' [Ki HK]]]; eauto;*)
-(*        [by eapply val_base_stuck| |]; simplify_eq/=.*)
-(*      * (** e1 is of the form ([Resolve] e10 e11 v0) and e11 takes a base_step. *)*)
-(*        inversion Hhstp'; simplify_eq.*)
-(*        edestruct (IH K) as (?&?&?&?&?&Hpstp&?&?&?&?);*)
-(*          [rewrite !length_app /=; lia|done|by eapply base_step_not_stuck|];*)
-(*            simplify_eq/=.*)
-(*        apply base_reducible_prim_step in Hpstp; simpl in *;*)
-(*          last by rewrite /base_reducible /=; eauto 10.*)
-(*        epose (λ H, base_step_to_val _ _ _ (Val _) _ _ _ _ _ _ _ H Hpstp)*)
-(*          as Hhstv; edestruct Hhstv as [? ?%of_to_val]; [done|eauto|];*)
-(*          simplify_eq.*)
-(*        eexists _, _, _, _, _; repeat split;*)
-(*          first (by apply base_prim_step; econstructor; eauto); auto.*)
-(*        etrans.*)
-(*        { by apply (rtc_pure_step_ctx*)
-(*                      (fill [PairLCtx _; PairLCtx _; FstCtx; FstCtx])). }*)
-(*        apply projs_pure_steps.*)
-(*      * (** e1 is of the form ([Resolve] e10 v v0) and e10 takes a*)
-(*           (non-base) prim_step. *)*)
-(*        rewrite fill_app in Hrs; simplify_eq/=.*)
-(*        edestruct (IH K) as (?&?&?&?&?&Hpstp&Hprstps&?&?&?);*)
-(*          [rewrite !length_app; lia|done| |].*)
-(*        { change (fill_item Ki) with (fill [Ki]).*)
-(*          by rewrite -fill_app; eapply prim_step_not_stuck, Ectx_step. }*)
-(*        simplify_eq/=.*)
-(*        change (fill_item Ki) with (fill [Ki]) in Hpstp.*)
-(*        rewrite -fill_app in Hpstp.*)
-(*        eapply base_reducible_prim_step_ctx in Hpstp as [e2'' [He2'' Hpstp]];*)
-(*          last by eexists _; eauto.*)
-(*        simplify_eq/=.*)
-(*        eexists _, _, _, _, _; repeat split.*)
-(*        -- apply (fill_prim_step [ResolveLCtx _ _ _]); eapply Ectx_step; eauto.*)
-(*        -- simpl; rewrite fill_app in Hprstps.*)
-(*           by apply (rtc_pure_step_ctx*)
-(*                    (fill [PairLCtx _; PairLCtx _; FstCtx; FstCtx])).*)
-(*    + (** e1 is of the form ([Resolve] e1_ e1_2 v) and e1_2 takes a prim_step. *)*)
-(*      repeat*)
-(*        match goal with*)
-(*        | H : erase_expr ?e = ?e' |- _ =>*)
-(*          progress*)
-(*            match e' with*)
-(*            | fill _ _ => idtac*)
-(*            | _ => destruct e; simplify_eq/=*)
-(*            end*)
-(*        end.*)
-(*      apply (prim_step_matched_by_erased_steps_ectx [ResolveMCtx _ _]).*)
-(*      apply IH; [rewrite !length_app /=; lia|done|*)
-(*                 by eapply (not_stuck_fill_inv (fill [ResolveMCtx _ _])); simpl].*)
-(*  - (** e1 is of the form ([Resolve] e1_ e1_2 e13) and e1_3 takes a prim_step. *)*)
-(*    apply (prim_step_matched_by_erased_steps_ectx [ResolveRCtx _ _]).*)
-(*    apply IH; [rewrite !length_app /=; lia|done|*)
-(*                 by eapply (not_stuck_fill_inv (fill [ResolveRCtx _ _])); simpl].*)
-(*Qed.*)
-
-(*Lemma erased_prim_step_prim_step e1 σ1 κ e2 σ2 efs:*)
-(*  prim_step (erase_expr e1) (erase_state σ1) κ e2 σ2 efs → not_stuck e1 σ1 →*)
-(*  prim_step_matched_by_erased_steps e1 σ1 e2 σ2 efs.*)
-(*Proof.*)
-(*  intros Hstp He1sf.*)
-(*  inversion Hstp as [K e1' e2' He1 ? Hhstp]; clear Hstp; simplify_eq/=.*)
-(*  set (len := length K); assert (length K = len) as Hlen by done; clearbody len.*)
-(*  revert K Hlen e1 He1 He1sf.*)
-(*  induction len as [m IHm]using lt_wf_ind; intros K Hlen e1 He1 He1sf;*)
-(*    simplify_eq.*)
-(*  destruct K as [|Ki K _] using rev_ind; simplify_eq/=.*)
-(*  { apply erased_base_step_base_step in Hhstp as (?&?&?&?&?&<-&?&<-).*)
-(*    eexists _, _, _, _, _; repeat split;*)
-(*      first (by apply base_prim_step); auto using rtc_refl. }*)
-(*  rewrite length_app in IHm; simpl in *.*)
-(*  rewrite fill_app /=; rewrite fill_app /= in He1.*)
-(*  eapply prim_step_matched_by_erased_steps_ectx_item; eauto; [].*)
-(*  { intros K' **; simpl in *. apply (IHm (length K')); auto with lia. }*)
-(*Qed.*)
-
-(*Lemma base_step_erased_prim_step_CAS v1 v2 σ l vl:*)
-(*  heap σ !! l = Some (Some vl) →*)
-(*  val_comparable vl v1 →*)
-(*  ∃ e2' σ2' ef', prim_step (CAS #l (erase_val v1)*)
-(*                             (erase_val v2)) (erase_state σ) [] e2' σ2' ef'.*)
-(*Proof.*)
-(*  intros Hl Hv.*)
-(*  destruct (bool_decide (vl = v1)) eqn:Heqvls.*)
-(*  - do 3 eexists; apply base_prim_step;*)
-(*      econstructor; [|by apply val_comparable_erase|by eauto].*)
-(*      by rewrite /erase_state /state_upd_heap /= lookup_erase_heap Hl.*)
-(*  - do 3 eexists; apply base_prim_step;*)
-(*        econstructor; [|by apply val_comparable_erase|by eauto].*)
-(*      by rewrite /erase_state /state_upd_heap /= lookup_erase_heap Hl.*)
-(*Qed.*)
-
-(*Lemma base_step_erased_prim_step_resolve e w σ :*)
-(*  (∃ e2' σ2' ef', prim_step (erase_expr e) (erase_state σ) [] e2' σ2' ef') →*)
-(*    ∃ e2' σ2' ef',*)
-(*    prim_step (erase_resolve (erase_expr e) #LitPoison (erase_val w)) (erase_state σ) [] e2' σ2' ef'.*)
-(*Proof.*)
-(*  intros (?&?&?&?).*)
-(*  by eexists _, _, _;*)
-(*    apply (fill_prim_step [PairLCtx _; PairLCtx _;FstCtx; FstCtx]).*)
-(*Qed.*)
-
-(*Lemma base_step_erased_prim_step_un_op σ op v v':*)
-(*  un_op_eval op v = Some v' →*)
-(*    ∃ e2' σ2' ef',*)
-(*    prim_step (Unop op (erase_val v)) (erase_state σ) [] e2' σ2' ef'.*)
-(*Proof.*)
-(*  do 3 eexists; apply base_prim_step; econstructor.*)
-(*  apply un_op_eval_erase; eauto.*)
-(*Qed.*)
-
-(*Lemma base_step_erased_prim_step_bin_op σ op v1 v2 v':*)
-(*  bin_op_eval op v1 v2 = Some v' →*)
-(*    ∃ e2' σ2' ef',*)
-(*    prim_step (Binop op (erase_val v1) (erase_val v2)) (erase_state σ) [] e2' σ2' ef'.*)
-(*Proof.*)
-(*  do 3 eexists; apply base_prim_step; econstructor.*)
-(*  apply bin_op_eval_erase; eauto.*)
-(*Qed.*)
-
-(*Lemma base_step_erased_prim_step_allocN σ l n v:*)
-(*  (0 < n)%Z →*)
-(*  (∀ i : Z, (0 ≤ i)%Z → (i < n)%Z → heap σ !! (l +ₗ i) = None) →*)
-(*    ∃ e2' σ2' ef',*)
-(*    prim_step (AllocN #n (erase_val v)) (erase_state σ) [] e2' σ2' ef'.*)
-(*Proof.*)
-(*  do 3 eexists; apply base_prim_step; econstructor; eauto.*)
-(*  intros; rewrite lookup_erase_heap_None; eauto.*)
-(*Qed.*)
-
-(*Lemma base_step_erased_prim_step_free σ l v :*)
-(*  heap σ !! l = Some (Some v) →*)
-(*    ∃ e2' σ2' ef',*)
-(*    prim_step (Free #l) (erase_state σ) [] e2' σ2' ef'.*)
-(*Proof.*)
-(*  intros Hw. do 3 eexists; apply base_prim_step; econstructor.*)
-(*  rewrite /erase_state /state_upd_heap /= lookup_erase_heap Hw; eauto.*)
-(*Qed.*)
-
-(*Lemma base_step_erased_prim_step_load σ l v:*)
-(*  heap σ !! l = Some (Some v) →*)
-(*    ∃ e2' σ2' ef',*)
-(*    prim_step (! #l) (erase_state σ) [] e2' σ2' ef'.*)
-(*Proof.*)
-(*  do 3 eexists; apply base_prim_step; econstructor.*)
-(*  rewrite /erase_state /state_upd_heap /= lookup_erase_heap.*)
-(*  by destruct lookup; simplify_eq.*)
-(*Qed.*)
-
-(*Lemma base_step_erased_prim_step_xchg σ l v w :*)
-(*  heap σ !! l = Some (Some v) →*)
-(*    ∃ e2' σ2' ef',*)
-(*    prim_step (Xchg #l (erase_val w)) (erase_state σ) [] e2' σ2' ef'.*)
-(*Proof.*)
-(*  intros Hl. do 3 eexists; apply base_prim_step; econstructor.*)
-(*  rewrite /erase_state /state_upd_heap /= lookup_erase_heap Hl; eauto.*)
-(*Qed.*)
-
-(*Lemma base_step_erased_prim_step_store σ l v w :*)
-(*  heap σ !! l = Some (Some v) →*)
-(*    ∃ e2' σ2' ef',*)
-(*    prim_step (#l <- erase_val w) (erase_state σ) [] e2' σ2' ef'.*)
-(*Proof.*)
-(*  intros Hw. do 3 eexists; apply base_prim_step; econstructor.*)
-(*  rewrite /erase_state /state_upd_heap /= lookup_erase_heap Hw; eauto.*)
-(*Qed.*)
-
-(*Lemma base_step_erased_prim_step_FAA σ l n n':*)
-(*  heap σ !! l = Some (Some #n) →*)
-(*    ∃ e2' σ2' ef',*)
-(*    prim_step (FAA #l #n') (erase_state σ) [] e2' σ2' ef'.*)
-(*Proof.*)
-(*  intros Hl.*)
-(*  do 3 eexists; apply base_prim_step. econstructor.*)
-(*  by rewrite /erase_state /state_upd_heap /= lookup_erase_heap Hl.*)
-(*Qed.*)
-
-(*(***)
-(*[Resolve] is translated as a projection out of a triple.*)
-(*Therefore, when resolve takes a base step, the erasure of [Resolve] takes a*)
-(*prim step inside the triple.*)
-(**)*)
-(*Lemma base_step_erased_prim_step e1 σ1 κ e2 σ2 ef:*)
-(*  base_step e1 σ1 κ e2 σ2 ef →*)
-(*    ∃ e2' σ2' ef',*)
-(*    prim_step (erase_expr e1) (erase_state σ1) [] e2' σ2' ef'.*)
-(*Proof.*)
-(*  induction 1; simplify_eq/=;*)
-(*    eauto using base_step_erased_prim_step_CAS,*)
-(*                base_step_erased_prim_step_resolve,*)
-(*                base_step_erased_prim_step_un_op,*)
-(*                base_step_erased_prim_step_bin_op,*)
-(*                base_step_erased_prim_step_allocN,*)
-(*                base_step_erased_prim_step_free,*)
-(*                base_step_erased_prim_step_load,*)
-(*                base_step_erased_prim_step_store,*)
-(*                base_step_erased_prim_step_xchg,*)
-(*                base_step_erased_prim_step_FAA;*)
-(*    by do 3 eexists; apply base_prim_step; econstructor.*)
-(*Qed.*)
-
-(*Lemma reducible_erased_reducible e σ :*)
-(*  reducible e σ →*)
-(*  reducible (erase_expr e) (erase_state σ).*)
-(*Proof.*)
-(*  intros (?&?&?&?&Hpstp); simpl in *.*)
-(*  inversion Hpstp; simplify_eq/=.*)
-(*  rewrite erase_ectx_expr.*)
-(*  edestruct base_step_erased_prim_step as (?&?&?&?); first done; simpl in *.*)
-(*  eexists _, _, _, _; eapply fill_prim_step; eauto.*)
-(*Qed.*)
-
-(*Lemma pure_step_tp_safe t1 t2 e1 σ :*)
-(*  (∀ e2, e2 ∈ t2 → not_stuck e2 σ) →*)
-(*  pure_steps_tp t1 (erase_exprs t2) →*)
-(*  e1 ∈ t1 → not_stuck e1 (erase_state σ).*)
-(*Proof.*)
-(*  intros Ht2 Hpr [i He1]%elem_of_list_lookup_1.*)
-(*  eapply Forall2_lookup_l in Hpr as [e2' [He2' Hpr]]; simpl in *; eauto.*)
-(*  rewrite /erase_exprs list_lookup_fmap in He2'.*)
-(*  destruct (t2 !! i) eqn:He2; simplify_eq/=.*)
-(*  apply elem_of_list_lookup_2, Ht2 in He2.*)
-(*  clear -Hpr He2.*)
-(*  inversion Hpr as [|??? [? _]]; simplify_eq.*)
-(*  - destruct He2 as [[? ?%of_to_val]|]; simplify_eq/=; first by left; eauto.*)
-(*    by right; apply reducible_erased_reducible.*)
-(*  - right; eauto using reducible_no_obs_reducible.*)
-(*Qed.*)
-
-Definition erased_step ρ1 ρ2 :=
-  ∃ κ ϕ,
-  step ρ1 κ ρ2 ϕ.
-
-Lemma erasure e σ :
-  adequate e σ →
-  adequate (erase_expr e) (erase_state σ).
-Proof.
-  intros H.
-  cut (
-    ∀ t2 σ2,
-    rtc erased_step ([erase_expr e], erase_state σ) (t2, σ2) →
-      ∃ t2' t2'' σ2',
-      rtc erased_step ([e], σ) (t2'', σ2') ∧
-      t2' = erase_exprs t2'' ∧
-      σ2 = erase_state σ2' ∧
-      Forall2 (rtc pure_step) t2 t2'
-  ). {
-    intros Hreach; split; simpl in *.
-    - intros ? ? ? Hrtc; edestruct (Hreach _ _ Hrtc) as
-          (t2'&t2''&σ2'&Hos&Ht2'&Hσ2&Hptp); simplify_eq/=.
-      apply Forall2_cons_inv_l in Hptp as (oe&t3&Hoe%rtc_pure_step_val&_&?);
-        destruct t2''; simplify_eq/=.
-      apply erase_to_val in Hoe as (?&?%of_to_val&?); simplify_eq.
-      pose proof (adequate_result _ _ _ _ Hade _ _ _ Hos); eauto.
-    - intros ? ? ? Hs Hrtc He2; edestruct (Hreach _ _ Hrtc) as
-          (t2'&t2''&σ2'&Hos&Ht2'&Hσ2&Hptp); simplify_eq/=.
-      eapply pure_step_tp_safe; [|done..].
-      intros e2' He2'.
-      apply (adequate_not_stuck _ _ _ _ Hade _ _ _ eq_refl Hos He2').
+  intros He Hσ Hadequate (𝑒s, 𝜎) H𝑠𝑡𝑒𝑝s.
+  eapply (erase_relation_steps ([e], σ)) in H𝑠𝑡𝑒𝑝s as ((es, σ') & (Hes & Hrel & ?) & Hsafe%Hadequate); last first.
+  { split_and!; first split; try done.
+    - apply Forall_singleton. done.
+    - apply Forall2_cons. done.
   }
-  intros t2 σ2 [n Hstps]%rtc_nsteps; simpl in *; revert t2 σ2 Hstps.
-  induction n as [|n IHn].
-  { intros t2 σ2 Hstps; inversion Hstps; simplify_eq /=.
-    repeat econstructor. }
-  intros t2 σ2 Hstps.
-  apply nsteps_inv_r in Hstps as [[t3 σ3] [Hstps Hρ]]; simpl in *.
-  destruct (IHn _ _ Hstps) as (t2'&t2''&σ2'&Hostps&?&?&Hprstps); simplify_eq.
-  edestruct @erased_step_pure_step_tp as [[? Hint]|Hext]; simplify_eq/=;
-    eauto 10; [|done..].
-  destruct Hext as (i&ei&t2'&efs&e'&κ&Hi1&Ht2&Hpstp);
-    simplify_eq/=.
-  rewrite /erase_exprs list_lookup_fmap in Hi1.
-  destruct (t2'' !! i) as [eio|] eqn:Heq; simplify_eq/=.
-  edestruct erased_prim_step_prim_step as
-    (eio' & σ3 & κ' & efs' & ee & Heiopstp & Hprstps' & ?&?&?); first done;
-    last simplify_eq/=.
-  { eapply adequate_not_stuck; eauto using elem_of_list_lookup_2. }
-  eexists _, _, _; repeat split.
-  { etrans; first done.
-    apply rtc_once; eexists.
-    eapply step_insert; eauto. }
-  rewrite /erase_exprs fmap_app.
-  rewrite list_fmap_insert/=.
-  apply Forall2_app; last done.
-  apply Forall2_same_length_lookup; split.
-  { apply Forall2_length in Hprstps; rewrite length_fmap in Hprstps.
-    by rewrite !length_insert length_fmap. }
-  intros j x y.
-  destruct (decide (i = j)); simplify_eq.
-  { rewrite !list_lookup_insert ?length_fmap; eauto using lookup_lt_Some; [].
-    by intros ? ?; simplify_eq. }
-  rewrite !list_lookup_insert_ne // list_lookup_fmap.
-  intros ? ?.
-  eapply Forall2_lookup_lr; eauto.
-  by rewrite /erase_exprs list_lookup_fmap.
+  simplify.
+  rewrite Forall_lookup => i 𝑒 H𝑒s_lookup.
+  eapply Forall2_lookup_r in Hrel as (e' & Hes_lookup & H𝑠𝑡𝑒𝑝s); last done.
+  eapply Forall_lookup in Hsafe; last done.
+  apply rtc_inv in H𝑠𝑡𝑒𝑝s as [-> | (𝑒' & H𝑠𝑡𝑒𝑝 & _)].
+  - apply erase_not_stuck. done.
+  - eapply pure_step_not_stuck. done.
 Qed.
